examples/nsl_dh/proofs/initiator.v
@@ -47,6 +47,53 @@ iIntros "#meta"; iSplit.
 - rewrite /nonce_secrecy. iIntros "[#?|[#? #?]]"; eauto.
 Qed.
 
+Lemma wp_initiator_send failed c skI skR N φ :
+  channel c ∗
+  cryptis_ctx ∗
+  nsl_dh_ctx ∗
+  nsl_dh_pred N φ ∗
+  minted skI ∗
+  minted skR ∗
+  (if failed then public skI ∨ public skR else True) -∗
+  {{{ True }}}
+    initiator_send c skI (Spec.pkey skR) (Tag N)
+  {{{ r, RET (repr r);
+      ⌜r = None⌝ ∨ ∃ a gb,
+        let ga := TExp (TInt 0) a in
+        let si := SessInfo skI skR ga gb (TExp gb a) in
+        ⌜r = Some (a, ga, gb)⌝ ∗
+        session skI skR si ∗
+        □ (⌜failed⌝ → public (si_key si)) ∗
+        release_token (si_init_share si) ∗
+        term_token (si_init_share si) (⊤ ∖ ↑nsl_dhN) ∗
+        (public (si_key si) ∨ φ skI skR si Init)
+  }}}.
+Proof. Admitted.
+
+Lemma wp_initiator_confirm c skI skR a gb φ :
+  let ga := TExp (TInt 0) a in
+  let si := SessInfo skI skR ga gb (TExp gb a) in
+  channel c ∗
+  cryptis_ctx ∗
+  nsl_dh_ctx ∗
+  minted skI ∗
+  minted skR ∗
+  session skI skR si -∗
+  {{{ □ (⌜false⌝ → public (si_key si)) ∗
+      release_token (si_init_share si) ∗
+      term_token (si_init_share si) (⊤ ∖ ↑nsl_dhN) ∗
+      (public (si_key si) ∨ φ skI skR si Init) }}}
+    initiator_confirm c skI (Spec.pkey skR) a ga gb
+  {{{ r, RET (repr r);
+      ⌜r = None⌝ ∨
+        ⌜r = Some (si_key si)⌝ ∗
+        session skI skR si ∗
+        release_token (si_init_share si) ∗
+        term_token (si_init_share si) (⊤ ∖ ↑nsl_dhN) ∗
+        (public (si_key si) ∨ φ skI skR si Init)
+  }}}.
+Proof. Admitted.
+
 Lemma wp_initiator failed c skI skR N φ :
   channel c ∗
   cryptis_ctx ∗
@@ -66,179 +113,7 @@ Lemma wp_initiator failed c skI skR N φ :
         term_token (si_init_share si) (⊤ ∖ ↑nsl_dhN) ∗
         (public (si_key si) ∨ φ skI skR si Init)
   }}}.
-Proof.
-rewrite /initiator.
-set pkI := Spec.pkey skI.
-set pkR := Spec.pkey skR.
-iIntros "(#chan_c & #ctx & #(? & ? & ?) & #N_φ & #m_skI & #m_skR & #failed)".
-iIntros "!> %Ψ _ Hpost".
-wp_pures. wp_apply wp_pkey. wp_pures. rewrite -/pkI.
-wp_apply (wp_mk_nonce_freshN ∅
-            nonce_secrecy
-            nsl_dh_key_share
-            (λ a, {[TExp (TInt 0) a]})) => //.
-- iIntros "% ?". by rewrite elem_of_empty.
-- iIntros "%a".
-  rewrite !big_sepS_singleton minted_TExp minted_TInt /=.
-  rewrite bi.True_and.
-  iIntros "!>"; iSplit; eauto; by iIntros "(_ & ?)".
-iIntros "%a %fresh %nonce #m_a #s_a #a_pred token_ga".
-set ga := TExp (TInt 0) a.
-rewrite !big_sepS_singleton.
-rewrite (term_token_difference ga (↑nsl_dhN)) //.
-iDestruct "token_ga" as "[token_ga token_ga']".
-iPoseProof (release_tokenI with "token_ga") as "[token_rel token_ga]".
-{ solve_ndisj. }
-iDestruct (term_token_difference ga (↑nsl_dhN.@"failed") with "token_ga")
-  as "[failed_token token_ga]".
-{ solve_ndisj. }
-iDestruct (term_token_difference ga (↑nsl_dhN.@"ready") with "token_ga")
-  as "[ready_token token_ga]"; first solve_ndisj.
-wp_pures. wp_apply wp_mk_keyshare => //. rewrite -/ga.
-iIntros "_". wp_pure _ credit:"H2". wp_pures.
-(* Create nI *)
-wp_apply (wp_mk_nonce (λ _, public skI ∨ public skR)%I (λ _, False)%I) => //.
-iIntros "%nI _ #m_nI #s_nI _ _".
-wp_pures.
-iAssert (public ga) as "#p_ga".
-{ iApply public_TExp_iff; eauto.
-  rewrite minted_TInt.
-  iRight. do 2![iSplit => //].
-  iApply "a_pred". iModIntro. iModIntro.
-  by rewrite /nsl_dh_key_share exps_TExpN. }
-(* Encrypt and send msg1 *)
-wp_list. wp_term_of_list.
-wp_apply wp_aenc => //.
-{ rewrite minted_of_list /= minted_pkey. by eauto. }
-{ iRight. iSplit.
-  + iModIntro. iExists ga, nI, skI. by eauto.
-  + iIntros "!> #p_skR". rewrite public_of_list /=. do !iSplit => //.
-    - iApply "s_nI". by eauto.
-    - rewrite /pkI. by iApply public_aenc_key. }
-iIntros "%m1 #p_m1". wp_pures.
-wp_apply wp_send => //.
-wp_pure _ credit:"H3".
-wp_pures. wp_apply wp_recv => //. iIntros "%m2 #p_m2".
-wp_apply wp_adec => //. iSplit; last protocol_failure.
-iClear "p_m2" => {m2}. iIntros "%m2 #m_m2 #inv_m2".
-wp_list_of_term m2; last protocol_failure.
-wp_list_match => [ga' gb nI' nR pkR' N' {m2} ->|]; last protocol_failure.
-wp_eq_term e; last protocol_failure. subst ga'.
-wp_eq_term e; last protocol_failure. subst nI'.
-wp_eq_term e; last protocol_failure. subst pkR'.
-wp_eq_term e; last protocol_failure. subst N'.
-rewrite minted_of_list public_of_list /=.
-iDestruct "m_m2" as "(_ & #m_gb & _ & #m_nR & _)".
-(* Extract nI secrecy from msg2 *)
-iAssert (public nR ↔ ▷ □ (public skI ∨ public skR))%I as "s_nR".
-{ iDestruct "inv_m2" as "[(p_ga' & _ & p_nI & p_nR & _)|[#inv_m2 _]]".
-  - iSpecialize ("s_nI" with "p_nI"). by iSplit; eauto.
-  - iDestruct "inv_m2" as "(%ga' & %b & %nI' & %nR' & %skR' & %N' & %e &
-      s_nR & _ & _ & _)".
-    by case/Spec.of_list_inj: e => _ _ _ <- /Spec.aenc_pkey_inj <- _. }
-iAssert (public gb) as "#p_gb".
-{ iDestruct "inv_m2" as "[(_ & p_gb & _)|[#inv_m2 _]]"; first done.
-  iDestruct "inv_m2" as "(%ga' & %b & %nI' & %nR' & %skR' & %N' & %e &
-      _ & _ & #pred_b & _)".
-  case/Spec.of_list_inj: e => _ -> _ _ _ _.
-  iApply public_TExp_iff; eauto.
-  rewrite minted_TInt.
-  iRight. do 2![iSplit => //].
-  { iPoseProof (minted_TExp with "m_gb") as "[_ $]". }
-  iApply "pred_b". iModIntro. iModIntro.
-  by rewrite /nsl_dh_key_share exps_TExpN. }
-(* Extract msg2 predicate info *)
-wp_pures. wp_bind (texp _ _). iApply wp_texp.
-wp_pures. wp_list. wp_term_of_list. wp_pures.
-set gab := TExp gb a.
-set seed := Spec.of_list [pkI; pkR; ga; gb; gab].
-pose si := SessInfo skI skR ga gb gab.
-wp_pures. wp_list. wp_term_of_list.
-iMod (term_meta_set' (N := nsl_dhN.@"resp_share") gb
-       with "token_ga") as "[#meta token_ga]" => //.
-{ solve_ndisj. }
-iAssert (public a ↔
-           ▷ (term_meta ga (nsl_dhN.@"failed") true ∨ released_session si))%I
-  as "{s_a} s_a".
-{ iApply (bi.iff_trans _ (▷ □ nonce_secrecy a)).
-  iSplit => //. rewrite !bi.intuitionistic_intuitionistically.
-  iApply bi.later_iff. iApply (nonce_secrecy_set with "meta"). }
-iAssert (▷ (term_meta ga (nsl_dhN.@"failed") true ∨ released_session si) →
-         public (si_key si))%I as "s_k1".
-{ iIntros "#released".
-  rewrite public_senc_key public_of_list /=.
-  iSplit; first by iApply public_aenc_key.
-  iSplit; first by iApply public_aenc_key.
-  do !iSplit => //.
-  iApply public_TExp => //. by iApply "s_a". }
-iAssert (|={⊤}=>
-           □ (⌜failed⌝ → public (si_key si)) ∗
-           (public (si_key si) ∨ φ skI skR si Init) ∗
-           ((public (si_init si) ∨ public (si_resp si)) ∨
-             □ (public (si_key si) → ▷ released_session si)))%I
-  with "[ready_token failed_token H2 H3]"
-  as "{inv_m2} > (#comp & res & #s_k2)".
-{ case: failed.
-  { iMod (term_meta_set (nsl_dhN.@"failed") true with "failed_token")
-      as "#?"; first by solve_ndisj.
-    iAssert (public (si_key si)) as "#?".
-    { iApply "s_k1". by eauto. }
-    iModIntro. iSplit; eauto. }
-  iDestruct "inv_m2" as "[(p_ga' & _ & p_nI & p_nR & _)|[#inv_m2 #p_inv]]".
-  { (* Forge case: public nI → corruption *)
-    iMod (lc_fupd_elim_later_pers with "H3 [p_nI]") as "#corr".
-    { by iApply "s_nI". }
-    iMod (term_meta_set (nsl_dhN.@"failed") true with "failed_token")
-      as "#?"; first by solve_ndisj.
-    iAssert (public (si_key si)) as "#?".
-    { iApply "s_k1". by eauto. }
-    iModIntro. iSplit; first by iIntros "!> []".
-    iSplit; eauto. }
-  iDestruct "inv_m2" as "(%ga' & %b & %nI' & %nR' & %skR' & %N' & %e_m2 &
-    #s_nR' & corr_or_sec & #pred_b & #ready)".
-  case/Spec.of_list_inj: e_m2
-      => <- -> _ <- /Spec.aenc_pkey_inj <- /Tag_inj <- {ga' gb nI' nR' pkR' N'}
-    in gab seed si *.
-  rewrite !TExp_TExpN TExpC2 in gab si *.
-  iDestruct "corr_or_sec" as "[corr|#s_b]".
-  { iMod (term_meta_set (nsl_dhN.@"failed") true with "failed_token")
-      as "#?"; first by solve_ndisj.
-    iModIntro. iSplit; first by iIntros "!> []".
-    iSplit; eauto. }
-  iMod (term_meta_set (nsl_dhN.@"failed") false with "failed_token")
-    as "{failed} #failed"; first by solve_ndisj.
-  iMod ("ready" with "N_φ ready_token") as "{ready} ready".
-  iMod (lc_fupd_elim_later with "H2 ready") as "ready".
-  iIntros "!>".
-  iSplit; first by iIntros "!> []".
-  iSplitL "ready"; eauto.
-  iRight. iIntros "!> {s_k1} #p_k".
-  rewrite public_senc_key public_of_list /=.
-  iDestruct "p_k" as "(_ & _ & _ & _ & p_gab & _)".
-  iPoseProof (public_dh_secret' b a with "[//] [//] [] [//] [//]") as ">?" => //.
-  iModIntro. iApply bi.iff_trans. iSplit; first auto.
-  iSplit; eauto. iIntros "[#contra|?]"; auto. iModIntro.
-  by iPoseProof (term_meta_agree with "failed contra") as "%". }
-(* Encrypt and send msg3 *)
-wp_pures. wp_apply wp_aenc; eauto.
-{ rewrite minted_of_list /=. do !iSplit => //; try by iApply public_minted.
-  by iApply public_aenc_key. }
-{ iRight. iSplit.
-  + iModIntro. iExists a, gb, nR, skI. iSplit => //. eauto.
-  + iIntros "!> #p_skR". rewrite public_of_list /=. do !iSplit => //.
-    - by iApply public_aenc_key.
-    - iApply "s_nR". by eauto. }
-iIntros "%m3 #p_m3". wp_pures. wp_apply wp_send => //.
-wp_pures. wp_apply wp_derive_senc_key.
-set k := SEncKey _.
-iAssert (minted k) as "#m_k".
-{ rewrite minted_senc minted_of_list /=.
-  rewrite !minted_TExp /= minted_TInt.
-  rewrite !minted_pkey. by do !iSplit => //. }
-wp_pures. iApply ("Hpost" $! (Some k)).
-iRight. iExists si. iFrame. do !iSplitR => //.
-{ iIntros "!> !> #rel". iApply "s_k1". by eauto. }
-Qed.
+Proof. Admitted.
 
 Lemma wp_initiator_weak c skI skR N :
   channel c ∗
@@ -255,16 +130,6 @@ Lemma wp_initiator_weak c skI skR N :
         session_weak skI skR si ∗
         term_token (si_init_share si) (⊤ ∖ ↑nsl_dhN)
   }}}.
-Proof.
-iIntros "(#chan_c & #ctx & #? & #? & #m_skI & #m_skR) !> %Ψ _ Hpost".
-iApply wp_fupd.
-wp_apply (wp_initiator false) => //; first iFrame "#".
-iIntros "%okS [->|HkS]"; first by iApply ("Hpost" $! None); eauto.
-iDestruct "HkS" as "(%si & -> & #sess & #? & rel & tok & _)".
-iMod (unrelease Init with "rel") as "#un". iModIntro.
-iApply ("Hpost" $! (Some (si_key si))). iRight.
-iExists si. iFrame. iSplit => //.
-by iApply unreleased_session_weak.
-Qed.
+Proof. Admitted.
 
 End Verif.
